
- Geometric Distribution
	- Recall m$X \leadsto \operatorname{Geom}(P)$.
	1. Range of $x$ is $D_{x} = \{ 1, 2, 3, \dots \}$
	2. $P(x) = q^{x-1} P; \, x = 1, 2, 3, \dots$
	3. $\mathbb{E}(x) = \dfrac{1}{P}$.
		- **N.B.**: intuitive explanation with coin flip until first success
			- 1st coin: $P = 0.9$
			- 2nd coin: $P = 0.15$
			- you'd expect to flip less to get the probability of $0.9$
- Proof: (expectation of $X$)
	- $\mathbb{E}(x) = \sum_{x=1}^{\infty} x q^{x-1} P$
		- **N.B.**: $q = 1-p$
	- $\mathbb{E}(x) = \sum_{x=1}^{\infty} \frac{d}{dx} q^x P$
		- **N.B.**: $q^x$ is the derivative of $q$ wiht resp to x
		- $= \frac{d}{dq} \sum_{x=1}^{\infty} q^x P$.
		- $= P \frac{d}{dq}\left[ \sum_{x=1}^{\infty} q^x \right]$
		- $= P \left( \frac{d}{dq} (q + q^2 + \dots + ) \right)$
		- $=P \cdot \dfrac{d}{dq} \left( q \underbrace{ \left( 1 + q + q^2 + \dots \right) }_{ {1/(1-q)} } \right)$
			- **N.B.**: recall from calculus II: $\dfrac{1}{1-r}1 + r + r^2 + r^3 + \dots \quad \lvert r \rvert < 1$
		- $= P \cdot \frac{d}{dq} \left( \frac{q}{1-q} \right)$
			- **N.B.**: use quotient rule
		- $= P \cdot \dfrac{1(1-q) - (-1)q}{(1-q)^2} = P \dfrac{1-q+q}{(1-q)^2} = P \cdot \dfrac{1}{P^2} = \dfrac{1}{P}$ $\blacksquare$

4. $M_{x}(t) = \dfrac{Pe^t}{1 - qe^t}, t < -\ln q$
	- Proof
		- $M_{x}(t) = \mathbb{E}(e^{tx}) = \sum_{x=1}^{\infty} e^{tx} \cdot q^{x-1} P$
		- $= P \sum_{x=1}^{\infty} e^{tx} \cdot q^{x-1}$
		- $= P \sum_{x=1}^{\infty} e^{tx} \cdot q^x \cdot \frac{1}{q}$
		- $= \dfrac{P}{q} \sum_{x=1}^{\infty} e^{tx} q^x$
		- $= \dfrac{P}{q} \sum_{x=1}^{\infty} (qe^t)^x$
			- **N.B.**: more like a geometric sequence
				- think of $qe^t$ as $r$
				- as long as $r$ is $< 1$, you can proceed as follow
		- $= \dfrac{P}{q} \left( qe^t + (qe^t)^2 + \dots \right)$
		- $= \dfrac{P}{q} (qe^t) (1 + qe^t + (qe^t)^2 + \dots$
		- $= Pe^t \left( \frac{1}{1-qe^t} \right) = \dfrac{Pe^t}{1 - qe^t}$
			- **N.B.**: $qe^t < 1 \quad \ln e^t < \ln \frac{1}{q} \quad \boxed{ t < -\ln q }$
- take first derivative of \#4 and plug in 0
	- $M_{x}'(t) = \dfrac{Pe^t (1-qe^t) - (-qe^t)Pe^t}{(1-qe^t)^2}$
		- $= \dfrac{Pe^t - Pqe^{2t} +Pqe^{2t}}{(1-qe^t)^2} = \dfrac{Pe^t}{(1-qe^t)^2}$
	- $M_{x}'(0) = \dfrac{Pe^0}{(1-qe^0)^2}$
		- $= \dfrac{P}{P^2}$
		- $= \dfrac{1}{P} = \mathbb{E}(X)$.
	- **N.B.**: three way to get the expectation of $X$
		- to get the variance, need to take derivative to get $E(x^2)$ then plug into variance formula
	- $M_{x}''(t) = \dfrac{Pe^t (1-qe^t)^2 - 2(1-qe^t)^1(-qe^t)Pe^t}{(1-qe^t)^4}$
		- $= \dfrac{Pe^t (1-qe^t) + 2qe^t \cdot Pe^t}{(1-qe^t)^3}$
	- $M_{x}''(0) = \dfrac{Pe^0 (1-qe^0) + 2q e^0 P e^0}{(1-qe^0)^3} = \dfrac{P(1-q)+2Pq}{(1-q)^3} = \dfrac{P - Pq + 2Pq}{(1-q)^3}$
		- $= \dfrac{P + Pq}{P^3} = \dfrac{P(1 + q)}{P^2} = \mathbb{E}(x^2)$
			- **N.B.**: $\dfrac{P(1 + q)}{P^2}$ is the expectation of $x^2$

5. $\operatorname{Var}( X ) = \mathbb{E}(x^2) - (\mathbb{E}(x))^2$
	- $= \dfrac{1+q}{P^2} - \dfrac{1}{P^2}$
	- $\boxed{ \operatorname{Var}( X ) = \dfrac{q}{P^2} }$

6. $P(X > k) = q^k,$ where $k$ is an integer.
	- $\Rightarrow \sum_{x=k+1}^{\infty} P(X = x)$
	- $= \sum_{x=k+1}^{\infty} q^{x-1}P$
	- $= P \sum_{x=k+1}^{\infty} q^{x-1} = P(q^k + q^{k+1} + \dots) = P \cdot q^k \left( \underbrace{ 1+q + q^2 + \dots }_{ \frac{1}{1-q} }  \right)$
	- $= Pq^k \cdot \dfrac{1}{1-q} = P \cdot q^k \dfrac{1}{P} = q^k$

- **Example**: A couple wants to have kids until they have a boy and then stop.
	1. What is the probability they will have 4 kids?
	2. How many kids do you expect them to have?
	- Assume equal chance for boy and girl.
	
	- Answer:
		 - It is a geometric distribution problem.
			 - **N.B.**: need to identify what type of distribution you're dealing with as part of solving it
		- $P(X = x) = q^{x-1}P$.
		1. $P(X=4) = \left( \frac{1}{2} \right)^{4-1} \cdot \frac{1}{2} = \left( \frac{1}{2} \right)^4 = \frac{1}{16}$
		2. $\mathbb{E}(X) = \frac{1}{p} = \dfrac{1}{\frac{1}{2}} =  2$.

### Negative Binomial Distribution

- Neg binom distrib has parameter, number of successes $r$ 
	- keep flipping coin until the number of successes are attained (diff from geometric distribution when you stop at first success)
- $X \leadsto \operatorname{NB}(r = \text{\# successes}, P)$
	1. Range of $X$ is $D_{x} = \{ r, r+1, r + 2, \dots \}$
	- **N.B.**: since $x$ is random variable that counts number of success, the range is $r, r+1, r+2, \dots$
		- this is like a geometric experiment repeated $r$ times
		- $X = (r_{1}(P) + \dots + (r_{r}(P)$

- pmf of $x \leadsto \operatorname{NB}(r, P)$
	- **Example**: Flip a coin with probability of success $P$.
	- What is the probability the 3rd Head appears on the 10th flip?
	- **N.B.**: last one is forced to be head with probability $P$.
		- then the first 9 flips contain 2 heads in whichever order
		- 2 parts to the question, the $\dbinom{9}{2}$ is a binomial problem
	- $P(X = 10) = \dbinom{10-1}{3-1} P^{3-1} \cdot (1-P)^{(10-1)-(3-1)} \cdot P$.
